verif/btrees/verif_splitnode_part3.v
@@ -13,7 +13,6 @@ Require Import btrees_sep.
 Require Import btrees_spec.
 Require Import verif_newnode.
 Require Import verif_findindex.
-Require Import index.
 Require Import verif_splitnode_part0.
 
 Opaque Znth.
@@ -51,7 +50,7 @@ Lemma splitnode_main_ifelse_part2_proof:
    forall (H0 : numKeys n = Fanout)
       (H : node_integrity (btnode val ptr0 le false First Last nval)) 
       (k : key) (fri : Z) 
-      (HFRI : findRecordIndex n k = ip fri)
+      (HFRI : findRecordIndex n k = fri)
       (vnewnode : val)
       (H1 : vnewnode <> nullval)
      (nleft := btnode val ptr0 le false First false nval : node val)
@@ -101,6 +100,8 @@ Proof.
     intros. pose proof I.
     unfold splitnode_main_if_else_part2.
     abbreviate_semax.
+    subst fri.
+    set (fri := findRecordIndex n k) in *.
     Intros ent_end.
     deadvars!.
     pose (e:=keychild val ke ce).
@@ -146,6 +147,7 @@ SEP (mem_mgr gv; le_iter_sepcon (nth_first_le (insert_le le e) Middle);
       - Exists fri.
         Exists (le_to_list(skipn_le le fri) ++ ent_end0).
         entailer!.
+        set (fri := findRecordIndex n k) in *.
         rewrite le_split with (i:=fri) (le:=le) at 1.
         rewrite le_to_list_app.
         replace (nth_first_le (insert_le le e) fri) with (nth_first_le le fri).
@@ -154,7 +156,7 @@ SEP (mem_mgr gv; le_iter_sepcon (nth_first_le (insert_le le e) Middle);
         rewrite nth_first_app_same1. auto.
         rewrite numKeys_nth_first. auto.
         simpl in H0. rewrite H0. omega. unfold e. simpl. auto.
-        simpl in HFRI. rewrite <- HFRI. apply FRI_repr. auto.
+        apply FRI_repr. auto.
         simpl in H0. rewrite H0. omega.
       -                         (* loop body *)
         Intros i.
@@ -168,8 +170,8 @@ SEP (mem_mgr gv; le_iter_sepcon (nth_first_le (insert_le le e) Middle);
             unfold k_; rewrite ?Ptrofs.repr_unsigned.
             rewrite <- app_assoc. auto.
             unfold n in H0. simpl in H0. auto.      
-            unfold e. simpl. auto. unfold findRecordIndex in HFRI. unfold n in HFRI. auto.
-            rewrite FRI_repr with (key2:=k) by auto. rewrite <- HFRI. auto.
+            unfold e. simpl. auto. auto.
+            rewrite FRI_repr with (key2:=k) by auto. auto.
           } 
           rewrite HINSERT.
           assert(HENTRY: exists ei, nth_entry_le i (insert_le le e) = Some ei).
@@ -249,6 +251,7 @@ SEP (mem_mgr gv; le_iter_sepcon (nth_first_le (insert_le le e) Middle);
     {                           (* fri >= 8 *)
       forward.                  (* skip *)
       entailer!.
+      set (fri := findRecordIndex n k) in *.
       assert((Middle <=? fri)= true).
       { clear -H8. rewrite Middle_eq. apply Z.leb_le. omega. }
       unfold splitnode_left, n.
@@ -261,9 +264,10 @@ SEP (mem_mgr gv; le_iter_sepcon (nth_first_le (insert_le le e) Middle);
       Exists (le_to_list (skipn_le le Middle) ++ ent_end0).
       simpl. rewrite numKeys_nth_first.
       rewrite nth_first_insert with (k:=ke). cancel.
-      unfold e. simpl. auto. simpl in HFRI.
-      rewrite FRI_repr with (key2:=k). rewrite HFRI. simpl. rewrite Middle_eq. simpl.
-      unfold idx_to_Z, ip in *. omega.
+      unfold e. simpl. auto.
+      rewrite FRI_repr with (key2:=k). simpl. rewrite Middle_eq. simpl.
+      change (findRecordIndex' le k 0) with fri.
+      omega.
       auto. simpl in H0. rewrite numKeys_le_insert. rewrite H0. rewrite Middle_eq.
       rewrite Fanout_eq. omega.
     }
@@ -278,8 +282,8 @@ SEP (mem_mgr gv; le_iter_sepcon (nth_first_le (insert_le le e) Middle);
       unfold n in H0. simpl in H0. rewrite <- app_assoc. simpl. reflexivity.
       rep_omega.
       simpl in H0. rewrite H0. auto.
-      unfold e. simpl. auto. unfold findRecordIndex in HFRI. unfold n in HFRI. 
-      rewrite FRI_repr with (key2:=k) by auto. rewrite HFRI. auto.
+      unfold e. simpl. auto.
+      rewrite FRI_repr with (key2:=k) by auto. auto.
     } 
     rewrite HINSERT.
     
